programs/lean/Project/Mergesort/Proof.lean
@@ -6,6 +6,9 @@ import Project.Mergesort.CopySliceProof
 import Project.Mergesort.SplitAtProof
 import Project.Mergesort.VectorProof
 import Project.Mergesort.IteratorProof
+import Project.Mergesort.OutputIteratorProof
+import Project.Mergesort.FormatProof
+import Project.Mergesort.StringProof
 import Project.Mergesort.MergeFunctionProof
 import Project.Mergesort.SortFunctionProof
 import Project.Mergesort.TextProof
